I think local nominal "traditional" substitution currently has a bug

Tealeaves/Backends/Named/Named.v
@@ -31,21 +31,53 @@ Fixpoint fold_with_history {A B: Type}
 
 Section rw.
 
-  Context {A B: Type}
-    (f: list B * A -> B).
 
-  Lemma fold_with_history_nil:
-    fold_with_history f nil = nil.
-  Proof.
-    reflexivity.
-  Qed.
+  Context {A B: Type}.
 
-  Lemma fold_with_history_cons {a l}:
-    fold_with_history f (a :: l) =
-      f ([], a) :: fold_with_history (f ⦿ [f ([], a)]) l.
+  Section basic.
+
+    Context (f: list B * A -> B).
+
+    Lemma fold_with_history_nil:
+      fold_with_history f nil = nil.
+    Proof.
+      reflexivity.
+    Qed.
+
+    Lemma fold_with_history_cons {a l}:
+      fold_with_history f (a :: l) =
+        f ([], a) :: fold_with_history (f ⦿ [f ([], a)]) l.
+    Proof.
+      cbn.
+      reflexivity.
+    Qed.
+
+    Lemma fold_with_history_one {a}:
+      fold_with_history f ([a]) =
+        [f ([], a)].
+    Proof.
+      cbn.
+      reflexivity.
+    Qed.
+
+  End basic.
+
+  Lemma fold_with_history_app {l1 l2: list A}:
+    forall (f: list B * A -> B),
+      fold_with_history f (l1 ++ l2) =
+        fold_with_history f l1 ++
+          fold_with_history (f ⦿ fold_with_history f l1) l2.
   Proof.
-    cbn.
-    reflexivity.
+    induction l1 as [|a l1 IHl1]; intros.
+    - cbn. change (f ⦿ []) with (f ⦿ Ƶ).
+      now rewrite preincr_zero.
+    - rewrite <- List.app_comm_cons.
+      rewrite fold_with_history_cons.
+      rewrite fold_with_history_cons.
+      rewrite IHl1.
+      rewrite <- List.app_comm_cons.
+      rewrite preincr_preincr.
+      reflexivity.
   Qed.
 
 End rw.
@@ -106,17 +138,311 @@ Inductive Binding: Type :=
   Bound: list name -> name -> list name -> Binding
 | Unbound: list name -> Binding.
 
-Fixpoint get_binding_rec (discarded: list name)  (l: list name) (looking_for: name): Binding :=
+Fixpoint get_binding_rec_bound (looking_for: name) (prefix: list name) (postfix: list name) (l: list name):
+  Binding :=
+  match l with
+  | nil => Bound prefix looking_for postfix
+  | cons y ys =>
+      if looking_for == y
+      then get_binding_rec_bound looking_for (prefix ++ [looking_for] ++ postfix) [] ys
+      else get_binding_rec_bound looking_for (prefix) (postfix ++ [y]) ys
+  end.
+
+Fixpoint get_binding_rec_unbound (looking_for: name) (prefix: list name) (l: list name): Binding :=
+  match l with
+  | nil => Unbound prefix
+  | cons y ys =>
+      if looking_for == y
+      then get_binding_rec_bound looking_for prefix [] ys
+      else get_binding_rec_unbound looking_for (prefix ++ [y]) ys
+  end.
+
+Definition get_binding (ctx: list name) (v: name) :=
+  get_binding_rec_unbound v [] ctx.
+
+Section rw.
+
+
+  Section cons.
+
+    Context (looking_for: name).
+    Context (pre post: list name) (a: name).
+
+    Lemma get_binding_rec_unbound_cons_neq: forall l,
+        a <> looking_for ->
+        get_binding_rec_unbound looking_for pre (a :: l) =
+          get_binding_rec_unbound looking_for (pre ++ [a]) l.
+    Proof.
+      intros.
+      cbn.
+      destruct_eq_args looking_for a.
+    Qed.
+
+    Lemma get_binding_rec_unbound_cons_eq: forall l,
+        a = looking_for ->
+        get_binding_rec_unbound looking_for pre (a :: l) =
+          get_binding_rec_bound looking_for pre [] l.
+    Proof.
+      intros.
+      cbn.
+      destruct_eq_args looking_for a.
+    Qed.
+
+    Lemma get_binding_rec_bound_cons_neq: forall l,
+        a <> looking_for ->
+        get_binding_rec_bound looking_for pre post (a :: l) =
+          get_binding_rec_bound looking_for pre (post ++ [a]) l.
+    Proof.
+      intros.
+      cbn.
+      destruct_eq_args looking_for a.
+    Qed.
+
+    Lemma get_binding_rec_bound_cons_eq: forall l,
+        a = looking_for ->
+        get_binding_rec_bound looking_for pre post (a :: l) =
+          get_binding_rec_bound looking_for (pre ++ [a] ++ post) [] l.
+    Proof.
+      intros.
+      cbn.
+      destruct_eq_args looking_for a.
+    Qed.
+
+    Lemma get_binding_eq: forall l,
+        a = looking_for ->
+        get_binding (a :: l) looking_for =
+          get_binding_rec_bound looking_for [] [] l.
+    Proof.
+      intros.
+      cbn.
+      destruct_eq_args looking_for a.
+    Qed.
+
+    Lemma get_binding_neq: forall l,
+        a <> looking_for ->
+        get_binding (a :: l) looking_for =
+          get_binding_rec_unbound looking_for [a] l.
+    Proof.
+      intros.
+      cbn.
+      destruct_eq_args looking_for a.
+    Qed.
+
+  End cons.
+
+  Lemma get_binding_rec_general: forall (looking_for: name) pre' post' l,
+      ~ looking_for ∈ post' ->
+      exists (pre post: list name),
+        get_binding_rec_bound looking_for pre' post' l =
+          Bound pre looking_for post
+        /\ ~ looking_for ∈ post.
+  Proof.
+    introv Hanin.
+    generalize dependent pre'.
+    generalize dependent post'.
+    induction l; intros.
+    - exists pre' post'. cbn; auto.
+    - destruct (looking_for == a).
+      { rewrite get_binding_rec_bound_cons_eq; auto. }
+      { rewrite get_binding_rec_bound_cons_neq; auto.
+        specialize (IHl (post' ++ [a])).
+        assert (Hnlf: ~ looking_for ∈ (post' ++ [a])).
+        { rewrite element_of_list_app.
+          rewrite element_of_list_one.
+          firstorder.
+        }
+        specialize (IHl Hnlf).
+        specialize (IHl pre').
+        auto.
+      }
+  Qed.
+
+  Lemma get_binding_bound_general: forall (looking_for: name) pre' post' l,
+      ~ looking_for ∈ post' ->
+      exists (pre post: list name),
+        get_binding_rec_bound looking_for pre' post' l =
+          Bound pre looking_for post
+        /\ pre ++ [looking_for] ++ post = (pre' ++ [looking_for] ++ post' ++ l)
+        /\ ~ looking_for ∈ post.
+  Proof.
+    introv Hnin.
+    generalize dependent pre'.
+    generalize dependent post'.
+    induction l; intros.
+    - exists (pre': list name) (post':list name).
+      cbn. splits.
+      + auto.
+      + rewrite List.app_nil_r.
+        reflexivity.
+      + assumption.
+    - destruct_eq_args looking_for a.
+      + rewrite (get_binding_rec_bound_cons_eq a); auto.
+        specialize (IHl [] ltac:(firstorder) (pre' ++ [a] ++ post')).
+        destruct IHl as [pre [post [rest1 [rest2 rest3]]]].
+        exists pre post. splits.
+        * tauto.
+        * rewrite rest2. rewrite List.app_nil_l.
+          repeat rewrite <- List.app_assoc.
+          reflexivity.
+        * assumption.
+      + rewrite (get_binding_rec_bound_cons_neq); auto.
+        specialize (IHl (post' ++ [a])).
+        assert (Hnlf: ~ looking_for ∈ (post' ++ [a])).
+        { rewrite element_of_list_app.
+          rewrite element_of_list_one.
+          firstorder.
+        }
+        specialize (IHl Hnlf).
+        specialize (IHl pre').
+        destruct IHl as [pre [post [rest1 [rest2 rest3]]]].
+        exists pre post.
+        splits.
+        * assumption.
+        * rewrite rest2.
+          repeat rewrite <- List.app_assoc.
+          reflexivity.
+        * assumption.
+  Qed.
+
+  Lemma get_binding_spec_gen: forall l v pre',
+      ~ v ∈ pre' ->
+      {get_binding_rec_unbound v pre' l = Unbound (pre' ++ l) /\ ~ v ∈ (pre' ++ l)} +
+        {exists pre post: list name, get_binding_rec_unbound v pre' l =
+                                  Bound pre v post /\ (pre' ++ l = pre ++ [v] ++ post) /\ ~ v ∈ post}.
+  Proof.
+    intros.
+    unfold get_binding.
+    generalize dependent pre'.
+    induction l; intros pre' prenin.
+    - cbn. left. rewrite List.app_nil_r.
+      auto.
+    - destruct_eq_args v a.
+      + right.
+        rewrite get_binding_rec_unbound_cons_eq; auto.
+        specialize (get_binding_bound_general a pre' [] l ltac:(firstorder)).
+        intros [pre [post [rest1 [rest2 rest3]]]].
+        exists pre post. repeat rewrite List.app_nil_l in rest2.
+        auto.
+      + rewrite get_binding_rec_unbound_cons_neq; auto.
+        specialize (IHl (pre' ++ [a])).
+        rewrite <- List.app_assoc in IHl.
+        destruct IHl.
+        * rewrite element_of_list_app. firstorder.
+        * left.
+          assumption.
+        * right.
+          destruct e as [pre [post [rest1 [rest2 rest3]]]].
+          exists pre post. splits; auto.
+  Qed.
+
+  Lemma get_binding_spec: forall (l: list name) (v: name),
+      {get_binding l v = Unbound l /\ ~ v ∈ l} +
+        {exists pre post, get_binding l v = Bound pre v post  /\ l = pre ++ [v] ++ post /\ ~ v ∈ post}.
+  Proof.
+    intros.
+    unfold get_binding.
+    specialize (get_binding_spec_gen l v []); intro.
+    specialize (H ltac:(firstorder)).
+    rewrite List.app_nil_l in H.
+    auto.
+  Qed.
+
+
+  Lemma get_binding1: forall ctx v,
+      ~ (v ∈ ctx) -> get_binding ctx v = Unbound ctx.
+  Proof.
+    intros. destruct (get_binding_spec ctx v).
+    - tauto.
+    - enough (v ∈ ctx).
+      contradiction.
+      destruct e as [pre [post [rest1 [rest2 rest3]]]].
+      rewrite rest2.
+      autorewrite with tea_list. tauto.
+  Qed.
+
+End rw.
+
+
+Section rw.
+
+  #[local] Notation "'l'" := [ 1 ; 3; 4; 3; 2 ].
+
+  Compute get_binding l 1. (* [] 1 [3; 4; 3; 2] *)
+  Compute get_binding l 2. (* Bound [1; 3; 4; 3] 2 [] *)
+  Compute get_binding l 3. (* Bound [1; 3; 4] 3 [2] *)
+
+End rw.
+
+(*
+  Lemma get_binding_rec_unbound1: forall l1 l2 a,
+  get_binding_rec_unbound l1 [a] l2 = Unbound (l1 + l) ->
+  get_binding_rec_unbound [a] l2 = Unbound (l1 + l) ->
+  get_binding_rec_unbound v [a] l
+ *)
+
+
+(*
+
+  Fixpoint get_binding_rec (discarded: list name)  (l: list name) (looking_for: name): Binding :=
   match l with
   | nil => Unbound discarded
   | cons y ys =>
-      if looking_for == y
-      then Bound discarded y ys
-      else get_binding_rec (discarded ++ [y]) ys looking_for
+  if looking_for == y
+  then Bound discarded y ys
+  else get_binding_rec (discarded ++ [y]) ys looking_for
   end.
 
-Definition get_binding: list name -> name -> Binding :=
+  Fixpoint get_binding_rec (discarded: list name)  (l: list name) (looking_for: name): Binding :=
+  match l with
+  | nil => Unbound discarded
+  | cons y ys =>
+  if looking_for == y
+  then Bound discarded y ys
+  else get_binding_rec (discarded ++ [y]) ys looking_for
+  end.
+
+
+  Definition get_binding: list name -> name -> Binding :=
   get_binding_rec [].
+
+
+
+  Lemma get_binding_spec: forall (disc: list name) (l: list name) (v: name),
+  {get_binding_rec disc l v = Unbound (disc ++ l) /\ ~ v ∈ l} +
+  {exists pre post, get_binding_rec disc l v = Bound (disc ++ pre) v post  /\ l = pre ++ [v] ++ post /\ ~ v ∈ post}.
+  Proof.
+  intros.
+  induction l.
+  - cbn. left.
+  rewrite List.app_nil_r; split; auto.
+  - (* Lookup v in (a :: l) after discarding (disc). *)
+  cbn.
+  destruct_eq_args v a.
+  + right. destruct (IHl).
+  * exists (@nil name). exists l.
+  rewrite List.app_nil_r.
+  rewrite List.app_nil_l.
+  split. firstorder.
+  firstorder.
+  * destruct e as [pre [post [IH1 [IH2 IH3]]]].
+  exists (@nil name) post.
+  rewrite List.app_nil_r.
+  rewrite List.app_nil_l.
+  split; auto.
+  split; auto.
+  firstorder.
+
+  induction l.
+  { exists (@nil name) (@nil name).
+  rewrite List.app_nil_r.
+  rewrite List.app_nil_l.
+  split; auto.
+  }
+  { destruct
+  +
+
+  .
+ *)
 
 Section examples.
 
