Tealeaves/Backends/Named/NamedTraditional.v
@@ -14,6 +14,20 @@ Import List.ListNotations.
 Import Product.Notations.
 Import ContainerFunctor.Notations.
 
+Ltac step_set_test :=
+  match goal with
+  | H: ~ ?x ∈ ?t |- _ =>
+      let Hf := fresh "H" in
+      pose H as Hf;
+      rewrite <- SmartAtom.name_inb_iff_false in Hf;
+      progress (repeat rewrite Hf)
+  | H: ?x ∈ ?t |- _ =>
+      let Hf := fresh "H" in
+      pose H as Hf;
+      rewrite <- SmartAtom.name_inb_iff in Hf;
+      progress (repeat rewrite Hf)
+  end.
+
 Section alt.
 
   Context
@@ -32,7 +46,7 @@ Section alt.
 
 
     (* Given a substitution of x by u, encode the logic of what happens at <<current>> if <<history>> is the set of names
-     given to the binders so far *)
+       given to the binders so far *)
     Definition rename_binder_local_history:
       list name * name -> name :=
       fun '(history, b) =>
@@ -51,43 +65,38 @@ Section alt.
       destruct_eq_args x b.
     Qed.
 
-    Lemma rename_binder_local_history_rw2 {b}:
+    Lemma rename_binder_local_history_rw2 {hist b}:
+      b <> x ->
+      (b ∈ fv_u) ->
+      rename_binder_local_history (hist, b) = fresh (conflicts ++ hist ++ [b]).
+    Proof.
+      introv BneqX BinFVu.
+      unfold rename_binder_local_history.
+      destruct_eq_args x b.
+      rewrite <- SmartAtom.name_inb_iff in BinFVu.
+      rewrite BinFVu.
+      reflexivity.
+    Qed.
+
+    Lemma rename_binder_local_history_rw2' {b}:
       b <> x ->
       b ∈ fv_u ->
       rename_binder_local_history (nil, b) = fresh (conflicts ++ [b]).
     Proof.
       intros.
-      unfold rename_binder_local_history.
-      destruct_eq_args x b.
-      rewrite <- SmartAtom.name_inb_iff in H2.
-      rewrite H2.
-      rewrite List.app_nil_l.
-      reflexivity.
+      rewrite rename_binder_local_history_rw2; auto.
     Qed.
 
     Lemma rename_binder_local_history_rw3 {hist b}:
       b <> x ->
-      (b ∈ fv_u) ->
-      rename_binder_local_history (hist, b) = fresh (conflicts ++ hist ++ [b]).
-    Proof.
-      intros.
-      unfold rename_binder_local_history.
-      destruct_eq_args x b.
-      rewrite <- SmartAtom.name_inb_iff in H2.
-      rewrite H2.
-      reflexivity.
-    Qed.
-
-    Lemma rename_binder_local_history_rw4 {hist b}:
-      b <> x ->
       ~ (b ∈ fv_u) ->
       rename_binder_local_history (hist, b) = b.
     Proof.
-      intros.
+      introv BneqX BinFVu.
       unfold rename_binder_local_history.
       destruct_eq_args x b.
-      rewrite <- SmartAtom.name_inb_iff_false in H2.
-      rewrite H2.
+      rewrite <- SmartAtom.name_inb_iff_false in BinFVu.
+      rewrite BinFVu.
       reflexivity.
     Qed.
 
@@ -102,19 +111,18 @@ Section alt.
     Qed.
 
     Lemma ctx_to_history_cons1 {nm l}:
-      x <> nm ->
-      ~ (nm ∈ fv_u) ->
+      x = nm ->
       ctx_to_history (nm :: l) =
         nm :: fold_with_history (rename_binder_local_history ⦿ [nm]) l.
     Proof.
       intros.
       unfold ctx_to_history.
       rewrite fold_with_history_cons.
-      rewrite rename_binder_local_history_rw2; auto.
+      rewrite rename_binder_local_history_rw1; auto.
     Qed.
 
 
-    Lemma ctx_to_history_cons2 {nm l}:
+    Lemma ctx_to_history_cons_cons2 {nm l}:
       x <> nm ->
       (nm ∈ fv_u) ->
       ctx_to_history (nm :: l) =
@@ -123,36 +131,112 @@ Section alt.
       intros.
       unfold ctx_to_history.
       rewrite fold_with_history_cons.
-      rewrite rename_binder_local_history_rw3; auto.
+      rewrite rename_binder_local_history_rw2'; auto.
     Qed.
 
-    Lemma ctx_to_history_dist: forall l1 l2,
-      ctx_to_history (l1 ++ l2) = ctx_to_history l1 ++ ctx_to_history l2.
+    Lemma ctx_to_history_cons_rw3 {nm l}:
+      x <> nm ->
+      ~ (nm ∈ fv_u) ->
+      ctx_to_history (nm :: l) =
+        nm :: fold_with_history (rename_binder_local_history ⦿ [nm]) l.
     Proof.
       intros.
       unfold ctx_to_history.
-      induction l1.
-      reflexivity.
-      rewrite <- List.app_comm_cons.
+      rewrite fold_with_history_cons.
+      rewrite rename_binder_local_history_rw3; auto.
+    Qed.
+
+
+    Lemma ctx_to_history_app: forall l1 l2,
+        ctx_to_history (l1 ++ l2) =
+          ctx_to_history l1 ++
+            (fold_with_history (rename_binder_local_history ⦿ fold_with_history rename_binder_local_history l1) l2).
+    Proof.
+      intros.
       unfold ctx_to_history.
-      rewrite fold_with_history_cons.
-      rewrite fold_with_history_cons.
-      rewrite <- List.app_comm_cons.
-      fequal.
-    Abort.
+      rewrite fold_with_history_app.
+      reflexivity.
+    Qed.
 
 
     (* Name a binder to something else during substitution *)
     Definition rename_binder_local:
       list name * name -> name :=
       fun '(ctx, b) =>
-        if SmartAtom.name_inb x ctx (* Halt substitution early, we didnt' past where x appears in ctx *)
+        if SmartAtom.name_inb x ctx (* Halt substitution early, we didn't recurse where x appears in ctx *)
         then b
         else if x == b (* Else check if halt now *)
              then b (* This binder is the name of the free variable we're substituting, halt and leave binder alone *)
              else if SmartAtom.name_inb b fv_u (* Else check if need to rename *)
-             then (rename_binder_local_history (ctx_to_history ctx, b))
-             else b.
+                  then (rename_binder_local_history (ctx_to_history ctx, b))
+                  else b.
+
+    (* This binder is under an abstraction of the substituted variable, do nothing (subst halted earlier) *)
+    Lemma rename_binder_local_rw1: forall ctx b,
+        x ∈ ctx ->
+        rename_binder_local (ctx, b) = b.
+    Proof.
+      intros.
+      unfold rename_binder_local.
+      step_set_test.
+      reflexivity.
+    Qed.
+
+    (* This binder is equal to the variable begin substituted (subst is halting now) *)
+    Lemma rename_binder_local_rw2: forall ctx b,
+        ~ (x ∈ ctx) ->
+        x = b ->
+        rename_binder_local (ctx, b) = b.
+    Proof.
+      intros.
+      unfold rename_binder_local.
+      destruct_eq_args x b.
+      now step_set_test.
+    Qed.
+
+    (* This binder conflicts with the free variables of u, rename after computing its history from its context *)
+    Lemma rename_binder_local_rw3: forall ctx b,
+        ~ (x ∈ ctx) ->
+        x <> b ->
+        b ∈ fv_u ->
+        rename_binder_local (ctx, b) = (rename_binder_local_history (ctx_to_history ctx, b)).
+    Proof.
+      intros.
+      unfold rename_binder_local.
+      step_set_test.
+      destruct_eq_args x b.
+      step_set_test.
+      reflexivity.
+    Qed.
+
+    (* This is a bound variable that doesn't cause any conflicts, do nothing *)
+    Lemma rename_binder_local_rw4: forall ctx b,
+        ~ (x ∈ ctx) ->
+        x <> b ->
+        ~ (b ∈ fv_u) ->
+        rename_binder_local (ctx, b) = b.
+    Proof.
+      intros.
+      subst.
+      unfold rename_binder_local.
+      destruct (SmartAtom.name_inb x ctx); auto.
+      destruct_eq_args x b.
+      step_set_test.
+      reflexivity.
+    Qed.
+
+    Corollary rename_binder_local_rw5: forall ctx b,
+        ~ (b ∈ fv_u) ->
+        rename_binder_local (ctx, b) = b.
+    Proof.
+      intros.
+      unfold rename_binder_local.
+      destruct (SmartAtom.name_inb x ctx).
+      - reflexivity.
+      - destruct_eq_args x b.
+        step_set_test.
+        reflexivity.
+    Qed.
 
     Definition subst_local:
       list name * name -> T name name :=
@@ -160,18 +244,96 @@ Section alt.
         if SmartAtom.name_inb x ctx (* Halt substitution early *)
         then ret (T := T name) v
         else
-               match (get_binding ctx v) with
-               | Unbound _ =>
-                   if v == x
-                   then u
+          match (get_binding ctx v) with
+          | Unbound _ =>
+              if v == x
+              then u
+              else ret (T := T name) v
+          | Bound prefix _ _ =>
+              if v == x
+              then ret (T := T name) v
+              else if SmartAtom.name_inb v (fv_u)
+                   then ret (T := T name) (rename_binder_local_history (prefix, v))
+                   else ret (T := T name) (rename_binder_local_history (prefix, v))
+                            (*
                    else ret (T := T name) v
-               | Bound prefix _ _ =>
-                   if v == x
-                   then ret (T := T name) v
-                   else if SmartAtom.name_inb v (FV T u)
-                        then ret (T := T name) (rename_binder_local_history (prefix, v))
-                        else ret (T := T name) v
-               end.
+                             *)
+          end.
+
+
+    (* This variable is under an abstraction of the substituted variable, do nothing (subst halted earlier) *)
+    Lemma subst_local_rw1: forall ctx v,
+        x ∈ ctx ->
+        subst_local (ctx, v) = ret v.
+    Proof.
+      intros.
+      unfold subst_local.
+      step_set_test.
+      reflexivity.
+    Qed.
+
+    (* This variable is equal to the variable begin substituted, replace it *)
+    Lemma subst_local_rw2: forall ctx v,
+        ~ (x ∈ ctx) ->
+        x = v ->
+        subst_local (ctx, v) = u.
+    Proof.
+      intros.
+      unfold subst_local.
+      destruct_eq_args x v.
+      step_set_test.
+      rewrite get_binding1; auto.
+    Qed.
+
+    Lemma hmmm:forall ctx v,
+        ~ v ∈ ctx ->
+        v = (rename_binder_local_history (ctx_to_history ctx, v)).
+    Proof.
+      intros.
+    Abort.
+
+
+    (* This is a bound variable that  conflicts with the free variables of u,
+       rename it to match its binder *)
+    Lemma subst_local_rw3: forall ctx v,
+        ~ (x ∈ ctx) ->
+        x <> v ->
+        v ∈ fv_u ->
+        subst_local (ctx, v) = ret (rename_binder_local_history (ctx_to_history ctx, v)).
+    Proof.
+      intros.
+      unfold subst_local.
+      step_set_test.
+      destruct (get_binding_spec ctx v) as [Case1 | Case2].
+      { destruct Case1 as [hyp1 hyp2].
+        rewrite hyp1.
+        destruct_eq_args v x.
+        destruct_eq_args v x.
+        step_set_test.
+        fequal.
+
+      rewrite get_binding1.
+      destruct_eq_args x v.
+      step_set_test.
+      reflexivity.
+    Qed.
+
+    (* This is a bound variable that doesn't cause any conflicts, do nothing *)
+    Lemma subst_local_rw4: forall ctx v,
+        ~ (x ∈ ctx) ->
+        x <> v ->
+        ~ (v ∈ fv_u) ->
+        suvst_local (ctx, v) = v.
+    Proof.
+      intros.
+      subst.
+      unfold subst_local.
+      destruct (SmartAtom.name_inb x ctx); auto.
+      destruct_eq_args x b.
+      step_set_test.
+      reflexivity.
+    Qed.
+
 
     Definition subst_top
       (t: T name name): T name name :=
